Further work on defining the STLC, thanks to Adam Koprowski

Instance/Lambda.v
@@ -1,31 +1,26 @@
-Require Import Coq.Bool.Bool.
-Require Import Coq.omega.Omega.
-Require Import Coq.Program.Wf.
+Set Warnings "-notation-overridden".
+
+Require Import Category.Lib.
+Require Export Category.Theory.Functor.
 
 Generalizable All Variables.
+Set Primitive Projections.
+Unset Universe Polymorphism.
+Set Transparent Obligations.
 
-Inductive type : Type :=
-  | Func : type -> type -> type
-  | Ty : type.                 (* Ty = type given below by [var t] *)
+Set Boolean Equality Schemes.
+Set Decidable Equality Schemes.
+
+Inductive type : Set :=
+  | Ty : type
+  | Func : type -> type -> type.
+
+Notation "x --> y" := (Func x y) (at level 55, right associativity) : type_scope.
 
 Fixpoint typeD (var : type -> Type) (t : type) : Type :=
   match t with
   | Ty => var Ty
   | Func x y => typeD var x -> typeD var y
-  end.
-
-Inductive Scope (var : type -> Type) (t : type) : type -> Type :=
-  | Here : Scope var t t
-  | Next u : var u -> Scope var t u.
-
-Arguments Here {_ _}.
-Arguments Next {_ _ _} _.
-
-Fixpoint scope_map {var var' : type -> Type} (f : forall t, var t -> var' t)
-        {d ty} (e : Scope var d ty) : Scope var' d ty :=
-  match e with
-  | Here => Here
-  | Next x => Next (f _ x)
   end.
 
 (** The lambda calculus
@@ -39,10 +34,124 @@ Fixpoint scope_map {var var' : type -> Type} (f : forall t, var t -> var' t)
     referencing a bound variable of the wrong type is also a type error.
     The type of free variables is given by [var] at the outermost level. *)
 
-Inductive Lam (var : type -> Type) : type -> Type :=
-  | Var : forall t   : type, var t -> Lam var t
-  | Abs : forall d c : type, Lam (Scope var d) c -> Lam var (Func d c)
-  | App : forall d c : type, Lam var (Func d c) -> Lam var d -> Lam var c.
+Inductive preterm : Set :=
+  | Var (i : nat)
+  | Abs (d : type) (body : preterm)
+  | App (arg body : preterm).
+
+Notation "% x" := (Var x) (at level 20).
+Infix "@" := App (at level 25, left associativity).
+Notation "\ A => M" := (Abs A M) (at level 35).
+
+Reserved Notation "E |- Pt := A" (at level 60).
+
+Require Import Coq.Lists.List.
+
+Definition Env := list (option type).
+Definition EmptyEnv : Env := nil.
+Definition VarD E x (A : type) := nth_error E x = Some (Some A).
+Definition VarUD E x := nth_error E x = None \/
+                        nth_error E x = Some (None : option type).
+Notation "E |= x := A" := (VarD E x A) (at level 60).
+Notation "E |= x :!"   := (VarUD E x) (at level 60).
+
+Definition decl (A : type) E := Some A :: E.
+
+Infix "[#]" := decl (at level 20, right associativity).
+
+Inductive Typing : Env -> preterm -> type -> Set :=
+  | TVar: ∀ Γ x α,                            (* x : α ∈ Γ *)
+         Γ |= x := α                          (* --------- *)
+      -> Γ |- %x := α                         (* Γ ⊢ x : α *)
+
+  | TAbs: ∀ Γ α β t,                          (*  Γ ∪ {x : α} ⊢ t : β  *)
+         α [#] Γ |- t := β                    (* --------------------- *)
+      -> Γ |- \α => t := α --> β              (* Γ ⊢ λx : α. t : α → β *)
+
+  | TApp: ∀ Γ α β t u,                        (* Γ ⊢ t : α → β   Γ ⊢ u : α *)
+         Γ |- t := α --> β  ->  Γ |- u := α   (* ------------------------- *)
+      -> Γ |- t @ u := β                      (*       Γ ⊢ t u : β         *)
+
+  where "Γ |- t := α" := (Typing Γ t α).
+
+Record term : Set := mkterm {
+  env    : Env;
+  tm     : preterm;
+  ty     : type;
+  typing : Typing env tm ty
+}.
+
+Lemma Type_unique : ∀ Pt E T1 T2
+  (D1 : Typing E Pt T1) (D2 : Typing E Pt T2), T1 = T2.
+Proof.
+  intros.
+  generalize dependent E.
+  generalize dependent T1.
+  generalize dependent T2.
+  induction Pt; simpl; intros.
+  - inversion_clear D1.
+    inversion H; subst; clear H.
+    inversion_clear D2.
+    inversion H; subst; clear H.
+    rewrite H1 in H2.
+    now inversion_clear H2.
+  - inversion_clear D1.
+    inversion_clear D2.
+    f_equal.
+    now eapply IHPt; eauto.
+  - inversion_clear D1.
+    inversion_clear D2.
+    specialize (IHPt1 _ _ _ H H1).
+    specialize (IHPt2 _ _ _ H0 H2).
+    subst.
+    now inversion_clear IHPt1.
+Qed.
+
+Lemma typing_unique : ∀ E Pt T (D1 D2 : Typing E Pt T),
+  D1 = D2.
+Proof.
+  intros.
+  apply Eqdep_dec.eq_dep_eq_dec.
+    apply type_eq_dec.
+Admitted.
+
+Lemma term_eq : ∀ M N,
+  env M = env N -> tm M = tm N -> M = N.
+Proof.
+  intros.
+  destruct M, N; simpl in *; subst.
+  pose proof (Type_unique _ _ _ _ typing0 typing1); subst.
+  f_equal.
+  apply typing_unique.
+Qed.
+
+Theorem autoType E Pt :
+  { N : term | env N = E & tm N = Pt} +
+  { ~ exists N : term, env N = E /\ tm N = Pt}.
+Proof.
+(*
+  destruct ({ α : type & Typing E Pt α } + { ~ exists α : type, Typing E Pt α }).
+  generalize dependent E.
+
+  induction Pt; intros.
+  - left.
+    exists {| env := E; tm := %i; ty := Ty; typing := TVar _ _ _ |}.
+*)
+Abort.
+
+Inductive Scope (var : type -> Type) (t : type) : type -> Type :=
+  | Here : Scope var t t
+  | Next u : var u -> Scope var t u.
+
+Arguments Here {_ _}.
+Arguments Next {_ _ _} _.
+
+Fixpoint scope_map {var var' : type -> Type} (f : ∀ t, var t -> var' t)
+        {d ty} (e : Scope var d ty) : Scope var' d ty :=
+  match e with
+  | Here => Here
+  | Next x => Next (f _ x)
+  end.
 
 Arguments Var {var _} _.
 Arguments Abs {var _ _} _.
@@ -55,7 +164,7 @@ Fixpoint lam_size {var : type -> Type} {ty} (e : Lam var ty) : nat :=
   | App func arg => 1 + lam_size func + lam_size arg
   end.
 
-Fixpoint lam_map {var var' : type -> Type} (f : forall t, var t -> var' t)
+Fixpoint lam_map {var var' : type -> Type} (f : ∀ t, var t -> var' t)
          {ty} (e : Lam var ty) : Lam var' ty :=
   match e with
   | Var x => Var (f _ x)
@@ -64,7 +173,7 @@ Fixpoint lam_map {var var' : type -> Type} (f : forall t, var t -> var' t)
   end.
 
 Lemma lam_map_size {var var' : type -> Type}
-      (f : forall t, var t -> var' t) {ty} (e : Lam var ty) :
+      (f : ∀ t, var t -> var' t) {ty} (e : Lam var ty) :
   lam_size (lam_map f e) = lam_size e.
 Proof.
   generalize dependent var'.
@@ -74,8 +183,7 @@ Defined.
 (** Instantiating a bound variable is function application. *)
 
 Definition instantiate {var : type -> Type}
-           {d c} (v : var d) (e : Lam (Scope var d) c) :
-  Lam var c :=
+           {d c} (v : var d) (e : Lam (Scope var d) c) : Lam var c :=
   let go _ x :=
       match x with
       | Here => v
@@ -100,12 +208,11 @@ Ltac simpl_eq :=
          EqdepFacts.internal_eq_sym_internal in *.
 
 Program Fixpoint lamD {t : type} (var : type -> Type)
-        (e : Lam (typeD var) t)
-        {measure (lam_size e)} : typeD var t :=
+        (e : Lam (typeD var) t) {measure (lam_size e)} : typeD var t :=
   match e as e' in Lam _ t'
-  return forall H : t' = t, e' = rew <- H in e -> typeD var t' with
-  | Var x => fun _ _ => x
-  | Abs body => fun _ _ => fun arg => lamD var (instantiate arg body)
+  return ∀ H : t' = t, e' = rew <- H in e -> typeD var t' with
+  | Var x        => fun _ _ => x
+  | Abs body     => fun _ _ => fun arg => lamD var (instantiate arg body)
   | App func arg => fun _ _ => lamD var func (lamD var arg)
   end eq_refl eq_refl.
 Next Obligation.
@@ -127,8 +234,134 @@ Notation "\ x : t , e" :=
 
 (*
 Eval cbv beta iota delta zeta in
-    lamD (fun _ => unit) ((\x : Ty, ^Here) @ ^tt).
+    lamD (fun _ => Datatypes.unit) ((\x : Ty, ^Here) @ ^tt).
 
 Eval cbv beta iota delta zeta in
-    lamD (fun _ => nat) (@Abs _ Ty Ty (^(Next 5)) @ ^5).
+    lamD (fun _ => Datatypes.nat) (@Abs _ Ty Ty (^(Next 5%nat)) @ ^5%nat).
 *)
+
+Require Import Coq.Strings.String.
+
+Open Scope string_scope.
+
+Inductive ty : Type :=
+  | Name : string -> ty
+  | Func : ty → ty → ty.
+
+Inductive tm : Type :=
+  | var : string → tm
+  | app : tm → tm → tm
+  | abs : string → ty → tm → tm.
+
+Inductive value : tm → Prop :=
+  | v_abs : ∀ x T t,
+      value (abs x T t).
+
+Hint Constructors value.
+
+Reserved Notation "'[' x ':=' s ']' t" (at level 20).
+
+Fixpoint subst (x:string) (s:tm) (t:tm) : tm :=
+  match t with
+  | var x' =>
+      if string_dec x x' then s else t
+  | abs x' T t1 =>
+      abs x' T (if string_dec x x' then t1 else ([x:=s] t1))
+  | app t1 t2 =>
+      app ([x:=s] t1) ([x:=s] t2)
+  end
+
+where "'[' x ':=' s ']' t" := (subst x s t).
+
+ Inductive substi (s:tm) (x:string) : tm → tm → Prop :=
+  | s_var1 :
+      substi s x (var x) s
+  | s_var2 : ∀ x0,
+      substi s x (var x0) (var x0)
+  | s_abs : ∀ T t1,
+      substi s x (abs x T t1) s
+  | s_app : ∀ t1 t2,
+      substi s x (app t1 t2) s.
+
+Hint Constructors substi.
+
+Theorem substi_correct : ∀ s x t t',
+  [x:=s]t = t' ↔ substi s x t t'.
+Proof.
+  split; intros.
+  - induction t.
+    + simpl in H.
+      destruct (string_dec x s0); subst.
+        constructor.
+      constructor.
+Admitted.
+
+Reserved Notation "t1 '===>' t2" (at level 40).
+
+Inductive step : tm → tm → Prop :=
+  | ST_AppAbs : ∀ x T t12 v2,
+         value v2 →
+         (app (abs x T t12) v2) ===> [x:=v2]t12
+  | ST_App1 : ∀ t1 t1' t2,
+         t1 ===> t1' →
+         app t1 t2 ===> app t1' t2
+  | ST_App2 : ∀ v1 t2 t2',
+         value v1 →
+         t2 ===> t2' →
+         app v1 t2 ===> app v1 t2'
+
+where "t1 '===>' t2" := (step t1 t2).
+
+Hint Constructors step.
+
+(* Notation multistep := (multi step). *)
+(* Notation "t1 '===>*' t2" := (multistep t1 t2) (at level 40). *)
+
+Reserved Notation "Gamma '|-' t '∈' T" (at level 40).
+
+Inductive has_type : context → tm → ty → Prop :=
+  | T_Var : ∀ Gamma x T,
+      Gamma x = Some T →
+      Gamma |- tvar x ∈ T
+  | T_Abs : ∀ Gamma x T11 T12 t12,
+      Gamma & {{x --> T11}} |- t12 ∈ T12 →
+      Gamma |- tabs x T11 t12 ∈ TArrow T11 T12
+  | T_App : ∀ T11 T12 Gamma t1 t2,
+      Gamma |- t1 ∈ TArrow T11 T12 →
+      Gamma |- t2 ∈ T11 →
+      Gamma |- tapp t1 t2 ∈ T12
+  | T_True : ∀ Gamma,
+       Gamma |- ttrue ∈ TBool
+  | T_False : ∀ Gamma,
+       Gamma |- tfalse ∈ TBool
+  | T_If : ∀ t1 t2 t3 T Gamma,
+       Gamma |- t1 ∈ TBool →
+       Gamma |- t2 ∈ T →
+       Gamma |- t3 ∈ T →
+       Gamma |- tif t1 t2 t3 ∈ T
+
+where "Gamma '|-' t '∈' T" := (has_type Gamma t T).
+
+Hint Constructors has_type.
+
+Program Definition Lambda : Category := {|
+  obj     := type;
+  hom     := fun x y => ∀ var : type -> Type, Lam var (Func x y);
+  homset  := fun x y => {| equiv := fun f g =>
+    ∀ v, lamD v (f _) = lamD v (g _)
+  |};
+  id      := fun x => fun v => \ v : x, ^ Here;
+  compose := fun x y z f g => fun v => Abs (f (Scope v x) @ (g (Scope v x) @ (^ Here)));
+|}.
+Next Obligation.
+  equivalence.
+  congruence.
+Qed.
+Next Obligation.
+  proper.
+  rewrite H.
+  rewrite H0.
+  reflexivity.
+Qed.
+Next Obligation.
+  simpl.
